compiler/dafny/semantics/dafny_compilerProofScript.sml
@@ -32,7 +32,7 @@ Proof
   Cases_on ‘l’ \\ gvs []
 QED
 
-(* by magnus *)
+(* TODO Upstream? *) (* by magnus *)
 Theorem exists_mlstring:
   (∃x:mlstring. P x) ⇔ (∃s. P (strlit s))
 Proof
@@ -41,6 +41,7 @@ Proof
   \\ pop_assum $ irule_at Any
 QED
 
+(* TODO Upstream? *)
 Theorem isprefix_strcat:
   ∀s₁ s₂. isPrefix s₁ s₂ = ∃s₃. s₂ = s₁ ^ s₃
 Proof
@@ -64,6 +65,7 @@ Proof
   \\ last_x_assum drule_all \\ rpt strip_tac \\ gvs []
 QED
 
+(* TODO Already exists in freshenProof; make it Theorem *)
 Triviality lookup_append_eq:
   ∀n m₁ m₀.
     MEM n (MAP FST m₁) ⇒ lookup (m₁ ++ m₀) n = lookup m₁ n
@@ -73,6 +75,31 @@ Proof
   \\ Cases_on ‘ALOOKUP m₁ n’
   \\ gvs [ALOOKUP_NONE]
 QED
+
+(* TODO Already exists in freshenProof; make it Theorem *)
+Triviality freshen_rhs_exp_len_eq:
+  ∀m cnt rhss cnt' rhss'.
+    freshen_rhs_exps m cnt rhss = (cnt', rhss') ⇒
+    LENGTH rhss' = LENGTH rhss
+Proof
+  Induct_on ‘rhss’ \\ rpt strip_tac
+  \\ gvs [freshen_rhs_exps_def]
+  \\ rpt (pairarg_tac \\ gvs[])
+  \\ res_tac
+QED
+
+(* TODO Already exists in freshenProof; make it Theorem *)
+Triviality freshen_lhs_exp_len_eq:
+  ∀m cnt lhss cnt' lhss'.
+    freshen_lhs_exps m cnt lhss = (cnt', lhss') ⇒
+    LENGTH lhss' = LENGTH lhss
+Proof
+  Induct_on ‘lhss’ \\ rpt strip_tac
+  \\ gvs [freshen_lhs_exps_def]
+  \\ rpt (pairarg_tac \\ gvs[])
+  \\ res_tac
+QED
+
 (* ** *)
 
 Triviality map_add_fresh_every_is_fresh:
@@ -98,16 +125,177 @@ Proof
   \\ last_assum $ irule_at Any
 QED
 
+Triviality add_fresh_is_fresh:
+  add_fresh m cnt v = (cnt', m') ⇒ is_fresh (lookup m' v)
+Proof
+  disch_tac \\ gvs [add_fresh_def, lookup_def, is_fresh_def, isprefix_strcat]
+QED
+
+Definition get_param_names_def[simp]:
+  get_param_names (Method _ ins _ _ _ _ outs _ _) =
+    MAP FST ins ++ MAP FST outs ∧
+  get_param_names (Function _ ins _ _ _ _ _) = MAP FST ins
+End
+
+Triviality freshen_exp_is_fresh:
+  (∀m cnt e cnt' e'.
+     freshen_exp m cnt e = (cnt', e') ⇒ is_fresh_exp e') ∧
+  (∀m cnt es cnt' es'.
+     freshen_exps m cnt es = (cnt', es') ⇒
+     EVERY (λe. is_fresh_exp e) es')
+Proof
+  ho_match_mp_tac freshen_exp_ind
+  \\ rpt strip_tac
+  >~ [‘Var v’] >-
+   (gvs [freshen_exp_def]
+    \\ rpt (pairarg_tac \\ gvs [])
+    \\ gvs [is_fresh_def, lookup_def]
+    \\ CASE_TAC >- (simp [isprefix_thm])
+    \\ simp [isprefix_strcat])
+  >~ [‘Forall (v,ty) e’] >-
+   (gvs [freshen_exp_def]
+    \\ rpt (pairarg_tac \\ gvs [])
+    \\ imp_res_tac add_fresh_is_fresh)
+  \\ gvs [freshen_exp_def]
+  \\ rpt (pairarg_tac \\ gvs [])
+QED
+
+Triviality freshen_lhs_exp_is_fresh:
+  freshen_lhs_exp m cnt lhs = (cnt', lhs') ⇒ is_fresh_lhs_exp lhs'
+Proof
+  Cases_on ‘lhs’
+  >~ [‘VarLhs var’] >-
+   (rpt strip_tac
+    \\ gvs [is_fresh_lhs_exp, freshen_lhs_exp_def, lookup_def, is_fresh_def]
+    \\ CASE_TAC >- simp [isprefix_thm]
+    \\ simp [isprefix_strcat])
+  >~ [‘ArrSelLhs arr idx’] >-
+   (rpt strip_tac
+    \\ gvs [freshen_lhs_exp_def]
+    \\ rpt (pairarg_tac \\ gvs [])
+    \\ imp_res_tac (cj 1 freshen_exp_is_fresh) \\ simp [])
+QED
+
+Triviality freshen_lhs_exps_is_fresh:
+  ∀lhss m cnt cnt' lhss'.
+    freshen_lhs_exps m cnt lhss = (cnt', lhss') ⇒
+    EVERY (λe. is_fresh_lhs_exp e) lhss'
+Proof
+  Induct \\ simp [freshen_lhs_exps_def]
+  \\ rpt strip_tac
+  \\ rpt (pairarg_tac \\ gvs [])
+  \\ imp_res_tac freshen_lhs_exp_is_fresh \\ simp []
+  \\ res_tac
+QED
+
+Triviality freshen_rhs_exp_is_fresh:
+  freshen_rhs_exp m cnt rhs = (cnt', rhs') ⇒ is_fresh_rhs_exp rhs'
+Proof
+  Cases_on ‘rhs’
+  >~ [‘ExpRhs e’] >-
+   (simp [freshen_rhs_exp_def]
+    \\ rpt strip_tac
+    \\ rpt (pairarg_tac \\ gvs [])
+    \\ imp_res_tac (cj 1 freshen_exp_is_fresh))
+  >~ [‘ArrAlloc len init’] >-
+   (simp [freshen_rhs_exp_def]
+    \\ rpt strip_tac
+    \\ rpt (pairarg_tac \\ gvs [])
+    \\ imp_res_tac (cj 1 freshen_exp_is_fresh) \\ simp [])
+QED
+
+Triviality freshen_rhs_exps_is_fresh:
+  ∀rhss m cnt cnt' rhss'.
+    freshen_rhs_exps m cnt rhss = (cnt', rhss') ⇒
+    EVERY (λe. is_fresh_rhs_exp e) rhss'
+Proof
+  Induct \\ simp [freshen_rhs_exps_def]
+  \\ rpt strip_tac
+  \\ rpt (pairarg_tac \\ gvs [])
+  \\ imp_res_tac freshen_rhs_exp_is_fresh \\ simp []
+  \\ res_tac
+QED
+
+Triviality freshen_stmt_is_fresh:
+  ∀stmt m cnt cnt' stmt'.
+    freshen_stmt m cnt stmt = (cnt', stmt') ⇒ is_fresh_stmt stmt'
+Proof
+  Induct \\ rpt gen_tac
+  >~ [‘MetCall lhss name args’] >-
+   (simp [freshen_stmt_def]
+    \\ rpt strip_tac
+    \\ rpt (pairarg_tac \\ gvs [])
+    \\ imp_res_tac freshen_lhs_exps_is_fresh \\ simp []
+    \\ imp_res_tac (cj 2 freshen_exp_is_fresh))
+  >~ [‘Dec local scope’] >-
+   (simp [freshen_stmt_def]
+    \\ rpt strip_tac
+    \\ rpt (pairarg_tac \\ gvs [])
+    \\ imp_res_tac add_fresh_is_fresh \\ simp []
+    \\ res_tac)
+  >~ [‘Then stmt₀ stmt₁’] >-
+   (simp [freshen_stmt_def]
+    \\ rpt strip_tac
+    \\ rpt (pairarg_tac \\ gvs [])
+    \\ res_tac \\ simp [])
+  >~ [‘If tst thn els’] >-
+   (simp [freshen_stmt_def]
+    \\ rpt strip_tac
+    \\ rpt (pairarg_tac \\ gvs [])
+    \\ imp_res_tac (cj 1 freshen_exp_is_fresh) \\ simp []
+    \\ res_tac \\ simp [])
+  >~ [‘Assign ass’] >-
+   (simp [freshen_stmt_def]
+    \\ rpt strip_tac
+    \\ rpt (pairarg_tac \\ gvs [])
+    \\ EVERY (map imp_res_tac
+               [freshen_rhs_exp_len_eq, freshen_lhs_exp_len_eq,
+                freshen_rhs_exps_is_fresh, freshen_lhs_exps_is_fresh])
+    \\ simp [MAP_ZIP])
+  >~ [‘While grd invs decrs mods body’] >-
+   (simp [freshen_stmt_def]
+    \\ rpt strip_tac
+    \\ rpt (pairarg_tac \\ gvs [])
+    \\ EVERY (map imp_res_tac (CONJUNCTS freshen_exp_is_fresh))
+    \\ simp [] \\ res_tac)
+  >~ [‘Print e ty’] >-
+   (simp [freshen_stmt_def]
+    \\ rpt strip_tac
+    \\ rpt (pairarg_tac \\ gvs [])
+    \\ imp_res_tac freshen_exp_is_fresh)
+  >~ [‘Assert e’] >-
+   (simp [freshen_stmt_def]
+    \\ rpt strip_tac
+    \\ rpt (pairarg_tac \\ gvs [])
+    \\ imp_res_tac freshen_exp_is_fresh)
+  (* Return, Skip *)
+  \\ simp [freshen_stmt_def]
+QED
+
 Triviality freshen_member_is_fresh:
-  freshen_member member = fresh_member ⇒ is_fresh_member fresh_member
+  ALL_DISTINCT (get_param_names member) ⇒
+  is_fresh_member (freshen_member member)
 Proof
   disch_tac
-  \\ Cases_on ‘member’
+  \\ namedCases_on ‘member’
+       ["name ins reqs ens rds decrs outs mods body",
+        "name ins res_t reqs rds decrs body"]
   \\ gvs [freshen_member_def]
   \\ rpt (pairarg_tac \\ gvs [])
-  >-
-   (imp_res_tac UNZIP_LENGTH
-    \\ simp [MAP_ZIP]
+  \\ EVERY (map imp_res_tac
+               ((CONJUNCTS freshen_exp_is_fresh) @
+                [UNZIP_LENGTH, map_add_fresh_every_is_fresh,
+                 freshen_stmt_is_fresh]))
+  \\ gvs [MAP_ZIP, UNZIP_MAP, ALL_DISTINCT_APPEND]
+QED
+
+Triviality map_freshen_member_is_fresh:
+  EVERY (λmember. ALL_DISTINCT (get_param_names member)) members ⇒
+  EVERY is_fresh_member (MAP freshen_member members)
+Proof
+  Induct_on ‘members’ \\ simp []
+  \\ rpt strip_tac
+  \\ irule freshen_member_is_fresh \\ simp []
 QED
 
 (* *** *)
@@ -128,11 +316,16 @@ Proof
   \\ gvs [ZIP_EQ_NIL, UNZIP_EQ_NIL]
 QED
 
+Definition valid_members_def:
+  valid_members (Program members) =
+  EVERY (λmember. ALL_DISTINCT (get_param_names member)) members
+End
+
 Theorem correct_compile:
   ∀dfy_ck prog s' r_dfy cml_decs env_cml (t: 'ffi cml_state).
     evaluate_program dfy_ck T prog = (s', r_dfy) ∧
     compile prog = INR cml_decs ∧
-    has_main prog ∧ has_basic_cons env_cml ∧
+    has_main prog ∧ valid_members prog ∧ has_basic_cons env_cml ∧
     0 < dfy_ck ∧ t.clock = dfy_ck ∧ ExnStamp t.next_exn_stamp = ret_stamp ∧
     r_dfy ≠ Rstop (Serr Rtype_error) ⇒
     ∃ck t' m' r_cml.
@@ -147,6 +340,8 @@ Proof
   \\ irule_at (Pos last) correct_freshen_program \\ simp []
   \\ namedCases_on ‘prog’ ["members"]
   \\ simp [valid_prog_def, freshen_program_def, has_main_freshen]
+  \\ irule_at (Pos hd) map_freshen_member_is_fresh
+  \\ conj_tac >- (fs [valid_members_def])
 
   \\ cheat
 QED
